examples/subtype.ec
@@ -1,0 +1,94 @@
+(* ==================================================================== *)
+subtype 'a word (n : int) = {
+  w : 'a list | size w = n
+} + witness.
+
+op cat ['a] [n m : int] (x : {'a word n}) (y : {'a word m}) : {'a word (n+m)} =
+  x ++ y.
+
+==> (traduction)
+
+op cat ['a] (x : 'a word) (y : 'a word) : 'a word =
+  x ++ y.
+
+lemma cat_spec ['a] :
+  forall (n m : int) (x y : 'a word),
+    size x = n => size y = m => size (cat x y) = (n + m).
+
+op xor [n m : int] (w1 : {word n}) (w2 : {word m}) : {word (min (n, m))} =
+  ...
+
+lemma foo ['a] [n : int] (w1 w2 : {'a word n}) :
+  xor w1 w2 = xor w2 w1.
+
+op vectorize ['a] [n m : int] (w : {'a word (n * m)}) : {{'a word n} word m}.
+
+-> Keeping information in application? Yes
+   -> should provide a syntax for giving the arguments
+
+      {w : word 256}
+
+      vectorize<:int, n = 4> w ==> infer: m = 64
+
+-> What to do when the inference fails
+   1. we reject (most likely)
+   2. we open a goal
+
+-> In a proof script (apply: foo) or (rewrite foo)
+   1. inference des dépendances (n, m, ...)
+   2. décharger les conditions de bord (size w1 = n, size w2 = n)
+
+-> Goal
+      n : int
+      m : int
+     w1 : {word n}
+     w2 : {word m}
+   ====================================================================
+     E[xor (cat w1 w2) (cat w2 w1)]
+
+   rewrite foo
+
+      n : int
+      m : int
+     w1 : {word n}
+     w2 : {word m}
+   ====================================================================
+     E[xor (cat w2 w1) (cat w1 w2)]
+
+   under condition:
+     exists p . size (cat w1 w2) = p /\ size (cat w2 w1) = p.
+
+   ?p = size (cat w1 w2)
+   ?p = size (cat w2 w1)
+
+-> can be solved using a extended prolog-like engine
+    1. declarations of variables (w1 : {word n}) (w2 : {word m})
+    2. prolog-like facts from operators types (-> ELPI)
+    3. theories (ring / int)
+
+-> subtypes in procedures
+
+   We can only depend on operators / constants. I.e. the following
+   program should be rejected:
+
+   module M = {
+     var n : int
+
+     proc f(x : {bool word M.n}) = {
+     }
+   }
+
+   Question:
+     - What about dependent types in the type for results:
+         we reject programs if we cannot statically check the condition
+     - What about the logics? we have to patch them.
+
+(* ==================================================================== *)
+nth ['a] 'a -> 'a list -> int -> 'a
+
+ws : {word n} list
+
+nth<:word> witness ws 2 : word
+nth<:{word n}>
+
+coercion : 'a word n -> 'a list
